test/Trace.v
@@ -1,0 +1,78 @@
+From HTTP Require Import
+     TesterSpec.
+
+Definition tester_send {E} `{testerE -< E} : itree E (packetT id) :=
+  embed Tester__Send [] Conn__Server (0, [], []).
+
+Definition tester_recv {E} `{testerE -< E} : itree E (packetT id) :=
+  embed Tester__Recv Conn__Server.
+
+Definition same_status_code (p0 p1 : payloadT id) : bool :=
+  match p0, p1 with
+  | inr (Response (Status _ c0 _) _ _), inr (Response (Status _ c1 _) _ _) =>
+    c0 =? c1
+  | _, _ => false
+  end%N.
+
+Definition echo0 : itree stE void :=
+  ITree.forever
+    ('(Packet s0 d0 p0) <- tester_send;;
+     '(Packet s1 d1 p1) <- tester_recv;;
+     if (d1 = s0?) &&& (s1 = d0?) &&& same_status_code p0 p1
+     then ret tt
+     else throw "Message mismatch").
+
+Definition payload (sc : status_code) : payloadT id :=
+  inr $ Response (status_line_of_code sc) [] None.
+
+Definition trace0 : list traceT :=
+  [Trace__Out $ Packet (Conn__User 0) Conn__Server $ payload 0;
+   Trace__In  $ Packet Conn__Server (Conn__User 0) $ payload 0].
+
+Goal is_trace echo0 trace0 = true.
+Proof. reflexivity. Qed.
+
+Goal accepts (backtrack echo0) trace0 = true.
+Proof. reflexivity. Qed.
+
+Definition trace1 : list traceT :=
+  [Trace__Out $ Packet (Conn__User 0) Conn__Server $ payload 0;
+   Trace__Out $ Packet (Conn__User 1) Conn__Server $ payload 1;
+   Trace__In  $ Packet Conn__Server (Conn__User 0) $ payload 0;
+   Trace__In  $ Packet Conn__Server (Conn__User 1) $ payload 1].
+
+Goal is_trace echo0 trace1 = false.
+Proof. reflexivity. Qed.
+
+Goal accepts (backtrack echo0) trace1 = false.
+Proof. reflexivity. Qed.
+
+Definition echo1 : itree stE void :=
+  (rec-fix loop l :=
+     b <- trigger Decide;;
+     if b : bool
+     then
+       pkt <- tester_send;;
+       call (pkt :: l)
+     else
+       pkt <- tester_recv;;
+       let '(Packet s1 d1 p1) := pkt in
+       match pick (fun pkt0 =>
+                     let 'Packet s0 d0 p0 := pkt0 in
+                     (d1 = s0?)
+                       &&& (s1 = d0?)
+                       &&& same_status_code p0 p1) l with
+       | Some (_, l') => call l'
+       | None => throw $ to_string pkt ++ " not found in:" ++ CRLF ++ list_to_string l
+       end) [].
+
+Goal is_trace echo1 trace0 = true.
+Proof. reflexivity. Qed.
+
+Goal accepts (backtrack echo1) trace0 = true.
+Proof. reflexivity. Qed.
+
+Goal is_trace echo1 trace1 = true.
+Proof. reflexivity. Qed.
+
+Compute accepts' bigNumber (backtrack echo1) trace1.
